

1

$$f_{\xi}(x, y) = \frac{e^{-2|y|}}{\pi(1+x^2)}$$

$$x \in [-\infty; +\infty]$$

$$y \in [-\infty; +\infty]$$

$$\begin{aligned} \frac{4}{\pi} \int_0^{\infty} \int_0^{\infty} \frac{e^{-2y}}{1+x^2} dx dy &= \int_0^{\infty} e^{-2y} \arctan(x) dy = \\ &= \int_0^{\infty} e^{-2y} \left(\frac{\pi}{2} - 0 \right) dy = -\frac{4 \cdot \pi}{\pi \cdot 2} \frac{e^{-2y}}{2} \Big|_0^{\infty} = 0 + 1 = 1 \end{aligned}$$

Звернемся

(2)

a)	η	-1	0	1
	P	$\frac{11}{24}$	$\frac{1}{4}$	$\frac{7}{24}$

	ξ	-1	1
	P	$\frac{1}{2}$	$\frac{1}{2}$

$$b) 1) E(\xi, \eta) = \begin{pmatrix} -1 \\ -1 \end{pmatrix} \cdot \frac{1}{8} + \begin{pmatrix} -1 \\ 1 \end{pmatrix} \cdot \frac{1}{3} + \begin{pmatrix} 0 \\ -1 \end{pmatrix} \cdot \frac{1}{12} + \begin{pmatrix} 0 \\ 1 \end{pmatrix} \cdot \frac{1}{6} + \begin{pmatrix} 1 \\ -1 \end{pmatrix} \cdot \frac{7}{24} =$$

$$= \begin{pmatrix} -\frac{1}{8} \\ -\frac{1}{8} \end{pmatrix} + \begin{pmatrix} -\frac{1}{3} \\ \frac{1}{3} \end{pmatrix} + \begin{pmatrix} 0 \\ -\frac{1}{12} \end{pmatrix} + \begin{pmatrix} 0 \\ \frac{1}{6} \end{pmatrix} + \begin{pmatrix} \frac{7}{24} \\ -\frac{7}{24} \end{pmatrix} = \begin{pmatrix} -\frac{1}{6} \\ 0 \end{pmatrix}$$

$$2) \text{cov}(\xi; \eta) = (-1 + \frac{1}{6}) \cdot (-1 - 0) \cdot \frac{1}{8} + (-1 + \frac{1}{6}) \cdot (1 - 0) \cdot \frac{1}{3} + (0 + \frac{1}{6}) \cdot (-1 - 0) \cdot \frac{1}{12} +$$

$$+ (0 + \frac{1}{6}) \cdot (1 - 0) \cdot \frac{1}{6} + (1 + \frac{1}{6}) \cdot (-1 - 0) \cdot \frac{7}{24} = -\frac{5}{6} (-1) \cdot \frac{1}{8} + (-\frac{5}{6} \cdot 1 \cdot \frac{1}{3}) +$$

$$+ \frac{1}{6} \cdot (-1) \cdot \frac{1}{12} + \frac{1}{6} \cdot 1 \cdot \frac{1}{6} + \frac{1}{6} (-1) \cdot \frac{7}{24} = \frac{5}{6 \cdot 8} + (-\frac{5}{6 \cdot 3}) + (-\frac{1}{6 \cdot 12}) +$$

$$+ \frac{1}{6} \cdot \frac{1}{6} + (-\frac{7}{6 \cdot 24}) = \frac{5}{48} - \frac{5}{18} - \frac{1}{72} + \frac{1}{36} - \frac{7}{6 \cdot 24} =$$

$$= \frac{1}{6} \left(\frac{5}{8} - \frac{5}{3} - \frac{1}{12} + \frac{1}{6} - \frac{7}{24} \right) = \frac{1}{6} \left(\frac{15 - 40 - 2 + 4 - 7}{24} \right) = -\frac{1}{6} \cdot \frac{30}{24} = -\frac{5}{24}$$

$$\text{cov}(\xi, \xi) = D(\xi) = (-1 - 0)^2 \cdot \frac{1}{8} + (-1 - 0)^2 \cdot \frac{1}{3} + (-1 - 0)^2 \cdot \frac{1}{12} + (1 - 0)^2 \cdot \frac{1}{6} +$$

$$+ (-1 - 0)^2 \cdot \frac{7}{24} = \frac{1}{8} + \frac{1}{3} + \frac{1}{12} + \frac{1}{6} + \frac{7}{24} = \frac{3 + 8 + 2 + 4 + 7}{24} = \frac{24}{24} = 1$$

$$\text{cov}(\eta, \eta) = (-1 + \frac{1}{6})^2 \cdot \frac{1}{8} + (-1 + \frac{1}{6})^2 \cdot \frac{1}{3} + (0 + \frac{1}{6})^2 \cdot \frac{1}{12} + (0 + \frac{1}{6})^2 \cdot \frac{1}{6} +$$

$$+ (1 + \frac{1}{6})^2 \cdot \frac{7}{24} = (-\frac{5}{6})^2 \cdot \frac{1}{8} + (-\frac{5}{6})^2 \cdot \frac{1}{3} + (\frac{1}{6})^2 \cdot \frac{1}{12} + (\frac{1}{6})^2 \cdot \frac{1}{6} + (\frac{7}{6})^2 \cdot \frac{7}{24} =$$

$$= \frac{25}{36 \cdot 8} + \frac{25}{36 \cdot 3} + \frac{1}{36 \cdot 12} + \frac{1}{36 \cdot 6} + \frac{49 \cdot 7}{36 \cdot 24} = \frac{1}{36} \left(\frac{25}{8} + \frac{25}{3} + \frac{1}{12} + \frac{1}{6} + \frac{49 \cdot 7}{24} \right) =$$

$$= \frac{1}{36} \left(\frac{25 \cdot 3 + 25 \cdot 8 + 2 + 4 + 49 \cdot 7}{24} \right) = \frac{26}{36}$$

$$Cov = \begin{pmatrix} \frac{26}{36} & \frac{5}{24} \\ \frac{5}{24} & 1 \end{pmatrix}$$

$$Cor = \begin{pmatrix} 1 & \frac{5}{4\sqrt{26}} \\ \frac{5}{4\sqrt{26}} & 1 \end{pmatrix}$$

с) $\frac{5}{4 \cdot \sqrt{26}} \approx 0,245$ - Величины относительно независимы и слабо коррелируют

3

a)

$f_1 \backslash f_2$	1	2	3	4
1	2	3	4	5
2	3	4	5	6
3	4	5	6	7
4	5	6	7	8

} φ_1

$f_1 \backslash f_2$	1	2	3	4
1	1	1	1	1
2	1	1	0	1
3	1	0	1	0
4	1	1	0	1

} φ_2

b)

$\varphi_2 \backslash \varphi_1$	2	3	4	5	6	7	8
0	0	0	0	$\frac{2}{16}$	0	$\frac{2}{16}$	0
1	$\frac{1}{16}$	$\frac{2}{16}$	$\frac{3}{16}$	$\frac{2}{16}$	$\frac{3}{16}$	0	$\frac{1}{16}$

$$\begin{aligned}
 c) 1) E(\varphi_1, \varphi_2) &= \binom{2}{1} \cdot \frac{1}{16} + \binom{3}{1} \cdot \frac{2}{16} + \binom{4}{1} \cdot \frac{3}{16} + \binom{5}{1} \cdot \frac{2}{16} + \binom{5}{1} \cdot \frac{2}{16} + \\
 &+ \binom{6}{1} \cdot \frac{3}{16} + \binom{7}{0} \cdot \frac{2}{16} + \binom{8}{1} \cdot \frac{1}{16} = \begin{pmatrix} \frac{2}{16} \\ \frac{1}{16} \end{pmatrix} + \begin{pmatrix} \frac{6}{16} \\ \frac{2}{16} \end{pmatrix} + \begin{pmatrix} \frac{12}{16} \\ \frac{3}{16} \end{pmatrix} + \begin{pmatrix} \frac{10}{16} \\ 0 \end{pmatrix} + \\
 &+ \begin{pmatrix} \frac{10}{16} \\ \frac{2}{16} \end{pmatrix} + \begin{pmatrix} \frac{18}{16} \\ \frac{3}{16} \end{pmatrix} + \begin{pmatrix} \frac{14}{16} \\ 0 \end{pmatrix} + \begin{pmatrix} \frac{8}{16} \\ \frac{1}{16} \end{pmatrix} = \begin{pmatrix} 5 \\ \frac{3}{4} \end{pmatrix}
 \end{aligned}$$

$$\begin{aligned}
 2) \operatorname{cov}(\varphi_1; \varphi_2) &= (2-5) \cdot \left(1 - \frac{3}{4}\right) \cdot \frac{1}{16} + (3-5) \cdot \left(1 - \frac{3}{4}\right) \cdot \frac{2}{16} + \\
 &+ (4-5) \cdot \left(1 - \frac{3}{4}\right) \cdot \frac{3}{16} + (5-5) \cdot \left(0 - \frac{3}{4}\right) \cdot \frac{2}{16} + (5-5) \cdot \left(1 - \frac{3}{4}\right) \cdot \frac{2}{16} + \\
 &+ (6-5) \cdot \left(1 - \frac{3}{4}\right) \cdot \frac{3}{16} + (7-5) \cdot \left(0 - \frac{3}{4}\right) \cdot \frac{2}{16} + (8-5) \cdot \left(1 - \frac{3}{4}\right) \cdot \frac{1}{16} = \\
 &= -\frac{3}{4 \cdot 16} + \left(-\frac{1}{16}\right) - \frac{3}{4 \cdot 16} + \frac{3}{4 \cdot 16} - \frac{3}{16} + \frac{3}{4 \cdot 16} = -\frac{1}{16} - \frac{3}{16} = -\frac{4}{16} = -\frac{1}{4}
 \end{aligned}$$

$$\begin{aligned}
 \operatorname{cov}(\varphi_1; \varphi_1) &= (2-5)^2 \cdot \frac{1}{16} + (3-5)^2 \cdot \frac{2}{16} + (4-5)^2 \cdot \frac{3}{16} + (6-5)^2 \cdot \frac{3}{16} + \\
 &+ (7-5)^2 \cdot \frac{2}{16} + (8-5)^2 \cdot \frac{1}{16} = \frac{9}{16} + \frac{4 \cdot 2}{16} + \frac{3}{16} + \frac{3}{16} + \frac{4}{16} + \frac{9}{16} = \\
 &= \frac{36}{16} = \frac{9}{4}
 \end{aligned}$$

$$\begin{aligned}
 \operatorname{cov}(\varphi_2; \varphi_2) &= \left(1 - \frac{3}{4}\right)^2 \cdot \frac{1}{16} + \left(1 - \frac{3}{4}\right)^2 \cdot \frac{2}{16} + \left(1 - \frac{3}{4}\right)^2 \cdot \frac{3}{16} + \left(0 - \frac{3}{4}\right)^2 \cdot \frac{2}{16} + \\
 &+ \left(1 - \frac{3}{4}\right)^2 \cdot \frac{2}{16} + \left(1 - \frac{3}{4}\right)^2 \cdot \frac{3}{4} + \left(0 - \frac{3}{4}\right)^2 \cdot \frac{2}{16} + \left(1 - \frac{3}{4}\right)^2 \cdot \frac{1}{16} = \\
 &= \frac{1}{16} \cdot \frac{1}{16} + \frac{1}{16} \cdot \frac{2}{16} + \frac{1}{16} \cdot \frac{3}{16} + \frac{9}{16} \cdot \frac{2}{16} + \frac{1}{16} \cdot \frac{2}{16} + \frac{1}{16} \cdot \frac{3}{4} + \frac{9}{16} \cdot \frac{2}{16} + \\
 &+ \frac{1}{16} \cdot \frac{1}{16} = \frac{1+2+3+18+2+3+18+1}{16^2} = \frac{48}{16^2}
 \end{aligned}$$

$$\operatorname{Cov matrix} = \begin{pmatrix} \frac{9}{4} & -\frac{1}{4} \\ -\frac{1}{4} & \frac{48}{16^2} \end{pmatrix}$$

$$3) \operatorname{Cor matrix} = \begin{pmatrix} 1 & \frac{-2}{3\sqrt{3}} \\ \frac{-2}{3\sqrt{3}} & 1 \end{pmatrix}$$

$$(4) \quad f_X = \frac{1}{2\pi}$$

$$E\eta_1 = \int_{-\pi}^{\pi} \frac{1}{2\pi} \cos \xi \, d\xi = 0$$

$$E\eta_2 = \int_{-\pi}^{\pi} \frac{1}{2\pi} \sin \xi \, d\xi = 0$$

$$D\eta_1 = \int_{-\pi}^{\pi} \cos^2 \xi \cdot \frac{1}{2\pi} \, d\xi = \frac{1}{2\pi} \cdot \cos \xi \sin \xi + \int_{-\pi}^{\pi} \sin^2 \xi \, d\xi =$$

$$\int 1 - \int \cos^2 \xi$$

$$= \frac{1}{2\pi} \cdot \frac{1}{2} (\xi + \cos \xi \cdot \sin \xi) \Big|_{-\pi}^{\pi} = \frac{-1 \cdot 0 + \pi}{4\pi} + \frac{-1 \cdot 0 - \pi}{4\pi} = \frac{1}{4} + \frac{1}{4} = \frac{1}{2}$$

$$D\eta_2 = \frac{1}{2\pi} \int_{-\pi}^{\pi} \sin^2 \xi \, d\xi = \frac{1}{2\pi} \cdot \frac{1}{2} \int_{-\pi}^{\pi} 1 - \cos 2\xi \, d\xi = \frac{1}{4\pi} \left(\xi - \frac{\sin 2\xi}{2} \right) \Big|_{-\pi}^{\pi} =$$

$$= \frac{\pi}{4\pi} - \frac{0}{2} - \frac{(-\pi)}{4\pi} - \frac{0}{2} = \frac{1}{4} + \frac{1}{4} = \frac{1}{2}$$

$$\text{cov}(\eta_1, \eta_2) = \int_{-\pi}^{\pi} \cos \xi \cdot \sin \xi \cdot \frac{1}{2\pi} \, d\xi = \frac{1}{2\pi} \frac{\sin^2 \xi}{2} \Big|_{-\pi}^{\pi} = 0$$

$$\text{cov-matrix}(\eta_1; \eta_2) = \begin{pmatrix} \frac{1}{2} & 0 \\ 0 & \frac{1}{2} \end{pmatrix}$$

$$\text{cor-matrix}(\eta_1; \eta_2) = \begin{pmatrix} 1 & 0 \\ 0 & 1 \end{pmatrix}$$

с) Корреляции нет, зависимость
есть ($\eta_1^2 + \eta_2^2 = 1$)

(5)

$$\xi \sim \text{Exp}_2$$

$$p(x) = \begin{cases} 0, & x < 0 \\ 2e^{-2x}, & x \geq 0 \end{cases}$$

$$\eta \sim U_{0,1}$$

$$p(x) = \begin{cases} 0, & x \notin [0,1] \\ 1, & x \in [0,1] \end{cases}$$



$$g(x) = 2e^{-2x}$$

$$g + p(x) = \int_0^x p(u) \cdot g(x-u) du$$

$$1) x > 1; \quad 2) x \leq 1$$

$$1) x > 1$$

$$\int_0^1 1 \cdot g(x-u) du = \int_0^1 2e^{-2(x-u)} du = 2 \cdot e^{-2x} \cdot \int_0^1 e^{2u} du = 2 \cdot e^{-2x} \cdot \frac{e^{2u}}{2} \Big|_0^1 =$$

$$= e^{-2x} (e^2 - 1)$$

$$2) x \leq 1$$

$$\int_0^x 1 \cdot g(x-u) du = \int_0^x 2 \cdot e^{-2(x-u)} du = e^{-2x} \cdot e^{2u} \Big|_0^x = e^{-2x} \cdot (e^{2x} - 1) =$$

$$= 1 - e^{-2x}$$

$$f_{\xi+\eta}(x) = \begin{cases} e^{-2x} (e^2 - 1), & x > 1 \\ 1 - e^{-2x}, & x \leq 1 \end{cases}$$